Finally got constraint enumeration working.

ADTExamples/QueryStructure/InsertQSSpecs.v
@@ -1,4 +1,4 @@
-Require Import List String Ensembles
+Require Import List String Ensembles Arith
         ADTNotation Program QueryStructureSchema QueryStructure.
 
 (* Definitions for updating query structures. *)
@@ -13,36 +13,44 @@ Definition RelationInsert
            (tup' : Tuple Heading) :=
   tup' = tup \/ R tup'.
 
+Definition SatisfiesSchemaConstraints
+           {qsSchema} Ridx tup :=
+  schemaConstraints (QSGetNRelSchema qsSchema Ridx) tup.
+
+Definition SatisfiesCrossRelationConstraints
+           {qsSchema} Ridx Ridx' tup R :=
+  BuildQueryStructureConstraints qsSchema Ridx Ridx' tup R.
+
 Definition QSInsertSpec
            (qs : QueryStructureHint)
-           (idx : _)
-           (tup : Tuple (schemaHeading (QSGetNRelSchema _ idx)))
+           (Ridx : _)
+           (tup : Tuple (schemaHeading (QSGetNRelSchema _ Ridx)))
            (qs' : QueryStructure qsSchemaHint)
 : Prop :=
   (* All of the relations with a different index are untouched
      by insert. *)
-  (forall idx',
-     idx <> idx' ->
-     GetRelation qsHint idx' = GetRelation qs' idx') /\
-  (* If [tup] is consistent with the schema constraints and the
-     cross-relation constraints, it is included in the relation
-     indexed by [idx] after insert; that relation is unspecified if
-     [tup] does not satisfy either set of constraints. *)
-  schemaConstraints (QSGetNRelSchema qsSchemaHint idx) tup
-  -> (forall idx',
-        BuildQueryStructureConstraints
-          qsSchemaHint idx idx' tup (GetRelation qsHint idx'))
-  -> (forall idx' tup',
-        idx' <> idx ->
-        BuildQueryStructureConstraints
-          qsSchemaHint idx' idx tup'
-          (RelationInsert tup (GetRelation qsHint idx)))
-  -> List.In (bindex idx) (map relName (qschemaSchemas qsSchemaHint))
-  -> (forall t, GetRelation qs' idx t <->
-               (RelationInsert tup (GetRelation qsHint idx) t)).
+  (forall Ridx',
+     Ridx <> Ridx' ->
+     GetRelation qsHint Ridx' = GetRelation qs' Ridx') /\
+  (* If [tup] is consistent with the schema constraints, *)
+  SatisfiesSchemaConstraints Ridx tup
+  (* and [tup] is consistent with the other tables per the cross-relation
+     constraints, *)
+  -> (forall Ridx', SatisfiesCrossRelationConstraints Ridx Ridx' tup (GetRelation qsHint Ridx'))
+  (* and each tuple in the other tables is consistent with the
+     table produced by inserting [tup] into the relation indexed by [Ridx], *)
+  -> (forall Ridx' tup',
+        Ridx' <> Ridx ->
+        SatisfiesCrossRelationConstraints
+          Ridx' Ridx tup'
+          (RelationInsert tup (GetRelation qsHint Ridx)))
+  (* [tup] is included in the relation indexed by [Ridx] after insert.
+   The behavior of insertion is unspecified otherwise. *)
+  -> (forall t, GetRelation qs' Ridx t <->
+               (RelationInsert tup (GetRelation qsHint Ridx) t)).
 
-Notation "'Insert' b 'into' idx " :=
-  (Bind (Pick (QSInsertSpec _ idx b))
+Notation "'Insert' b 'into' Ridx " :=
+  (Bind (Pick (QSInsertSpec _ Ridx b))
         (fun r' => Pick (fun r => r' = r)))
     (at level 80) : QuerySpec_scope.
 
@@ -53,31 +61,31 @@ Section InsertRefinements.
 
   (* Definition Insert_Valid_obligation_0 *)
   (*            (qsSchema : QueryStructureSchema) *)
-  (*            (idx idx' : string) *)
-  (*            (tup : Tuple (schemaHeading (GetNamedSchema qsSchema idx))) *)
-  (*            (idx_eq : idx = idx') *)
-  (* : Tuple (schemaHeading (GetNamedSchema qsSchema idx')). *)
+  (*            (Ridx Ridx' : string) *)
+  (*            (tup : Tuple (schemaHeading (GetNamedSchema qsSchema Ridx))) *)
+  (*            (Ridx_eq : Ridx = Ridx') *)
+  (* : Tuple (schemaHeading (GetNamedSchema qsSchema Ridx')). *)
   (* Proof. *)
-  (*   rewrite <- idx_eq. *)
+  (*   rewrite <- Ridx_eq. *)
   (*   eassumption. *)
   (* Defined. *)
 
   (* Arguments Insert_Valid_obligation_0 _ _ _ _ _ / _ . *)
 
   Lemma NamedSchema_eq_neq
-  : forall idx idx' a,
-      idx <> idx'
-      -> NamedSchema_eq a idx = true
-      -> NamedSchema_eq a idx' = false.
+  : forall Ridx Ridx' a,
+      Ridx <> Ridx'
+      -> NamedSchema_eq a Ridx = true
+      -> NamedSchema_eq a Ridx' = false.
   Proof.
     unfold NamedSchema_eq; destruct a; simpl.
     repeat find_if_inside; congruence.
   Qed.
 
   Lemma NamedSchema_eq_eq :
-    forall idx a,
-      relName a = idx
-      -> NamedSchema_eq a idx = true.
+    forall Ridx a,
+      relName a = Ridx
+      -> NamedSchema_eq a Ridx = true.
   Proof.
     intros; unfold NamedSchema_eq; destruct a; subst; simpl.
     caseEq (string_dec relName relName); eauto.
@@ -85,34 +93,38 @@ Section InsertRefinements.
 
   Hint Resolve AC_eq_nth_In AC_eq_nth_NIn NamedSchema_eq_neq
        NamedSchema_eq_eq crossConstr.
+  Hint Unfold SatisfiesCrossRelationConstraints
+       SatisfiesSchemaConstraints.
 
-  Program Definition Insert_Valid
-             (qsSchema : QueryStructureSchema)
-             (qs : QueryStructure qsSchema)
-             (idx : _)
-             (tup : Tuple (QSGetNRelSchemaHeading qsSchema idx))
-             (schConstr : schemaConstraints (QSGetNRelSchema qsSchema idx) tup)
-             (qsConstr : forall idx',
-                           BuildQueryStructureConstraints qsSchema idx idx' tup (GetRelation qs idx'))
-             (qsConstr' : forall idx',
-                            idx' <> idx ->
-                            forall tup',
-                            BuildQueryStructureConstraints qsSchema idx' idx tup'
-                                                           (RelationInsert tup (GetRelation qs idx)))
+  Program
+    Definition Insert_Valid
+    (qsSchema : QueryStructureSchema)
+    (qs : QueryStructure qsSchema)
+    (Ridx : _)
+    (tup : Tuple (QSGetNRelSchemaHeading qsSchema Ridx))
+    (schConstr : SatisfiesSchemaConstraints Ridx tup)
+    (qsConstr : forall Ridx',
+                  SatisfiesCrossRelationConstraints Ridx Ridx' tup (GetRelation qs Ridx'))
+    (qsConstr' : forall Ridx' tup',
+                   Ridx' <> Ridx ->
+                   SatisfiesCrossRelationConstraints
+                     Ridx' Ridx tup'
+                     (RelationInsert tup (GetRelation qs Ridx)))
   : QueryStructure qsSchema :=
     {| rels :=
-         replace_BoundedIndex _ (rels qs) idx
-                       {| rel := RelationInsert tup (GetRelation qs idx)|}
+         replace_BoundedIndex _ (rels qs) Ridx
+                       {| rel := RelationInsert tup (GetRelation qs Ridx)|}
     |}.
   Next Obligation.
     unfold RelationInsert in *; simpl in *; intuition; subst; eauto.
-    eapply ((ith_Bounded _ (rels qs) idx )); eassumption.
+    eapply ((ith_Bounded _ (rels qs) Ridx )); eassumption.
   Qed.
   Next Obligation.
-    destruct (BoundedString_eq_dec idx idx'); subst.
+    unfold SatisfiesCrossRelationConstraints in *;
+    destruct (BoundedString_eq_dec Ridx idx'); subst.
     - rewrite ith_replace_BoundIndex_eq; eauto.
     - rewrite ith_replace_BoundIndex_neq in *; eauto using string_dec.
-      destruct (BoundedString_eq_dec idx0 idx); subst.
+      destruct (BoundedString_eq_dec Ridx idx); subst.
       rewrite ith_replace_BoundIndex_eq in H0; simpl in *; eauto.
       unfold RelationInsert in H0; intuition; subst; eauto.
       rewrite ith_replace_BoundIndex_neq in H0; eauto using string_dec.
@@ -120,107 +132,696 @@ Section InsertRefinements.
 
   (*Definition DecideableSB (P : Prop) := {P} + {~P}.
 
-  Definition SchemaConstraints_dec qsSchema idx tup :=
-    DecideableSB (schemaConstraints (QSGetNRelSchema qsSchema idx) tup).
+  Definition SchemaConstraints_dec qsSchema Ridx tup :=
+    DecideableSB (schemaConstraints (QSGetNRelSchema qsSchema Ridx) tup).
 
-  Definition QSSchemaConstraints_dec qsSchema qs idx tup :=
+  Definition QSSchemaConstraints_dec qsSchema qs Ridx tup :=
     DecideableSB
-      (forall idx',
-         BuildQueryStructureConstraints qsSchema idx idx' tup (GetRelation qs idx')).
+      (forall Ridx',
+         BuildQueryStructureConstraints qsSchema Ridx Ridx' tup (GetRelation qs Ridx')).
 
-  Definition QSSchemaConstraints_dec' qsSchema qs idx tup :=
+  Definition QSSchemaConstraints_dec' qsSchema qs Ridx tup :=
     DecideableSB
-      (forall idx',
-         idx' <> idx ->
+      (forall Ridx',
+         Ridx' <> Ridx ->
          forall tup',
-                BuildQueryStructureConstraints qsSchema idx' idx tup'
-                                               (RelationInsert tup (GetRelation qs idx))). *)
+                BuildQueryStructureConstraints qsSchema Ridx' Ridx tup'
+                                               (RelationInsert tup (GetRelation qs Ridx))). *)
+
+  Definition decides (b : bool) (P : Prop) := if b then P else ~ P.
+
+  Lemma app_assoc
+        (A : Type)
+        (l m n : list A)
+  : l ++ m ++ n = (l ++ m) ++ n.
+  Proof.
+    induction l; simpl; auto.
+    rewrite IHl; reflexivity.
+  Defined.
+
+  Lemma app_cons {A : Set}:
+    forall (a : A) As As',
+      As ++ (a :: As') = (As ++ [a]) ++ As'.
+  Proof.
+    intros; rewrite <- app_assoc; reflexivity.
+  Defined.
+
+  Definition Ensemble_BoundedIndex_app_cons {A : Set}
+    (a : A)
+    (As As' : list A)
+    (P : Ensemble (BoundedIndex (As ++ a :: As')))
+  : Ensemble (BoundedIndex ((As ++ [a]) ++ As')).
+    rewrite app_cons in P; exact P.
+  Defined.
+
+  Definition BoundedIndex_app_cons {A : Set}
+    (a : A)
+    (As As' : list A)
+    (a' : BoundedIndex (As ++ a :: As'))
+  : BoundedIndex ((As ++ [a]) ++ As').
+    rewrite app_cons in a'; exact a'.
+  Defined.
+
+  Lemma ibound_BoundedIndex_app_cons {A : Set}
+    (a : A)
+    (As As' : list A)
+    (a' : BoundedIndex (As ++ a :: As'))
+  : ibound a' = ibound (BoundedIndex_app_cons a As As' a').
+  Proof.
+    unfold BoundedIndex_app_cons, eq_rec, eq_rect; simpl.
+    destruct (app_cons a As As'); reflexivity.
+  Qed.
+
+  Program Fixpoint Iterate_Ensemble_BoundedIndex'
+          {A : Set}
+          (Visited Remaining : list A)
+          (P : Ensemble (BoundedIndex (Visited ++ Remaining))) : Prop :=
+    match Remaining with
+        | [] => True
+        | a :: Remaining' =>
+          P {| bindex := a;
+               indexb := {| ibound := List.length Visited;
+                            boundi := _ |} |}
+          /\ Iterate_Ensemble_BoundedIndex' (Visited ++ (a :: nil)) Remaining' _
+    end.
+  Next Obligation.
+    clear P; induction Visited; simpl; auto.
+  Defined.
+  Next Obligation.
+    exact (Ensemble_BoundedIndex_app_cons _ _ _ P).
+  Defined.
+
+  Lemma Ensemble_BoundedIndex_app_equiv {A : Set}
+        (A_eq_dec : forall a a' : A, {a = a'} + {a <> a'})
+        (a : A) (As As' : list A)
+        (P : Ensemble (BoundedIndex (As ++ a :: As')))
+  : forall idx idx' n nth nth',
+      P {| bindex := idx; indexb := {| ibound := n; boundi := nth |}|} <->
+      Ensemble_BoundedIndex_app_cons a As As' P
+                                     {| bindex := idx'; indexb := {| ibound := n; boundi := nth' |}|}.
+  Proof.
+    split; unfold Ensemble_BoundedIndex_app_cons, BoundedIndex_app_cons, app_cons; simpl;
+    unfold eq_rec, eq_rect, eq_ind, eq_rect; destruct (app_assoc As [a] As'); auto;
+    generalize (indexb_ibound_eq
+            {| bindex := idx'; indexb := {| ibound := n; boundi := nth' |}|}
+            {| bindex := idx; indexb := {| ibound := n; boundi := nth |}|}
+            eq_refl); simpl; intros; subst;
+    erewrite (eq_proofs_unicity_Opt_A A_eq_dec _); eauto.
+  Qed.
+
+  Lemma BoundedIndex_app_cons_nth_eq {A : Set}
+        (A_eq_dec : forall a a' : A, {a = a'} + {a <> a'})
+  : forall
+      (As As' : list A)
+      a a' a'' n nth nth',
+      {| bindex := a; indexb := {| ibound := n; boundi := nth |}|} =
+      BoundedIndex_app_cons a' As As' {| bindex := a''; indexb := {| ibound := n; boundi := nth' |}|}.
+  Proof.
+    intros.
+    unfold BoundedIndex_app_cons, eq_rec, eq_rect; simpl.
+    destruct (app_cons a' As As').
+    generalize (indexb_ibound_eq
+            {| bindex := a''; indexb := {| ibound := n; boundi := nth' |}|}
+            {| bindex := a; indexb := {| ibound := n; boundi := nth |}|}
+               eq_refl); simpl; intros; subst.
+    erewrite (eq_proofs_unicity_Opt_A A_eq_dec nth'); reflexivity.
+  Qed.
+
+  Lemma Ensemble_BoundedIndex_nth_eq {A : Set}
+        (A_eq_dec : forall a a' : A, {a = a'} + {a <> a'})
+  : forall
+      (As : list A)
+      (P : Ensemble (BoundedIndex As))
+      a a' n nth nth',
+      P {| bindex := a; indexb := {| ibound := n; boundi := nth |}|} ->
+      P {| bindex := a'; indexb := {| ibound := n; boundi := nth' |}|}.
+  Proof.
+    intros;
+    generalize (indexb_ibound_eq
+            {| bindex := a'; indexb := {| ibound := n; boundi := nth' |}|}
+            {| bindex := a; indexb := {| ibound := n; boundi := nth |}|}
+               eq_refl); simpl; intros; subst.
+    erewrite (eq_proofs_unicity_Opt_A A_eq_dec nth'); eassumption.
+  Qed.
+
+  Lemma nth_error_app {A : Set} :
+    forall (a : A) (As As' : list A) n,
+      nth_error As n = Some a ->
+      nth_error (As ++ As') n = Some a.
+  Proof.
+    induction As; destruct n; simpl; intros; try discriminate; auto.
+  Defined.
+
+  Lemma Ensemble_nth_error_app
+        {A : Set}
+        (A_eq_dec : forall a a' : A, {a = a'} + {a <> a'})
+  : forall a As As' nth'
+      (P : Ensemble (BoundedIndex (As ++ (a :: As')))),
+      P {| bindex := a;
+           indexb := {| ibound := Datatypes.length As;
+                        boundi := nth' |} |}
+      -> (forall (a' : A) (n : nat) (nth : nth_error As n = Some a'),
+      P {| bindex := a';
+           indexb := {|
+                      ibound := n;
+                      boundi := nth_error_app As (a :: As') n nth |} |})
+      -> forall (a' : A) (n : nat) (nth : nth_error (As ++ [a]) n = Some a'),
+           Ensemble_BoundedIndex_app_cons a As As' P
+                                          {| bindex := a';
+                                             indexb := {| ibound := n;
+                                                          boundi := nth_error_app (As ++ [a]) As' n nth |} |}.
+  Proof.
+    intros.
+    destruct (eq_nat_dec (List.length As) n ); subst.
+    - rewrite (BoundedIndex_app_cons_nth_eq
+                 A_eq_dec As As' _ (List.length As)
+                 (nth_error_app (As ++ [a]%SchemaConstraints) As'
+                                (Datatypes.length As) nth)
+                 nth').
+      erewrite <- BoundedIndex_app_cons_nth_eq; eauto.
+      eapply Ensemble_BoundedIndex_app_equiv; eauto.
+    - assert (nth_error As n = Some a') by
+          (revert n nth n0; clear; induction As; destruct n; simpl; intros;
+           try congruence;
+           [destruct n; discriminate
+           | eauto]).
+      generalize (H0 _ _ H1); intros.
+      erewrite (BoundedIndex_app_cons_nth_eq
+                 A_eq_dec As As' _ n
+                 (nth_error_app (As ++ [a]%SchemaConstraints) As'
+                                n nth)).
+      erewrite <- BoundedIndex_app_cons_nth_eq; eauto.
+      eapply Ensemble_BoundedIndex_app_equiv; eauto.
+      Grab Existential Variables.
+      rewrite <- app_assoc; simpl; apply nth_error_app; eassumption.
+      apply nth_error_app; eassumption.
+      apply nth_error_app; eassumption.
+  Qed.
+
+  Lemma Iterate_Ensemble_equiv' {A : Set}
+        (A_eq_dec : forall a a' : A, {a = a'} + {a <> a'})
+  : forall (Remaining Visited : list A)
+           (P : Ensemble (BoundedIndex (Visited ++ Remaining))),
+      (forall a n (nth : nth_error Visited n = Some a),
+         P {| bindex := a;
+              indexb := {| ibound := n;
+                           boundi := nth_error_app _ _ _ nth |} |})
+      -> (Iterate_Ensemble_BoundedIndex' Visited Remaining P ->
+         forall idx, P idx).
+    intros; destruct idx as [idx [n nth_n] ]; simpl in *.
+    revert Visited P H H0 idx n nth_n; induction Remaining; simpl; intros.
+    - eapply Ensemble_BoundedIndex_nth_eq with (a := idx); auto.
+    - split_and.
+      assert (nth_error ((Visited ++ [a]%SchemaConstraints) ++ Remaining) n = Some idx)
+        as nth_n'
+          by (rewrite <- app_assoc; simpl; assumption).
+      generalize (IHRemaining _ _ (Ensemble_nth_error_app A_eq_dec _ _ _ P H1 H) H2 _ _ nth_n').
+      unfold Ensemble_BoundedIndex_app_cons, eq_rect; destruct (app_cons a Visited Remaining).
+      intros; erewrite (eq_proofs_unicity_Opt_A A_eq_dec nth_n); eauto.
+      Grab Existential Variables.
+      rewrite app_nil_r in nth_n; assumption.
+  Qed.
+
+  Lemma Iterate_Ensemble_equiv'' {A : Set}
+        (A_eq_dec : forall a a' : A, {a = a'} + {a <> a'})
+  : forall (Remaining Visited : list A)
+           (P : Ensemble (BoundedIndex (Visited ++ Remaining))),
+      (forall idx, P idx)
+      -> Iterate_Ensemble_BoundedIndex' Visited Remaining P.
+    induction Remaining; simpl; auto.
+    intros; split; eauto.
+    eapply IHRemaining; intros; eauto.
+    intros; destruct idx as [idx [n nth_n] ]; simpl in *.
+    eapply Ensemble_BoundedIndex_app_equiv; eauto.
+    Grab Existential Variables.
+    rewrite <- app_assoc in nth_n; simpl in nth_n; eassumption.
+  Qed.
+
+  Definition Iterate_Ensemble_BoundedIndex
+          (Bound : list string)
+          (P : Ensemble (BoundedIndex Bound)) : Prop :=
+    Iterate_Ensemble_BoundedIndex' [] Bound P.
+
+  Program Lemma refine_Iterate_Ensemble {A : Set}
+        (A_eq_dec : forall a a' : A, {a = a'} + {a <> a'})
+  : forall (As : list string)
+           (P : Ensemble (BoundedIndex As)),
+      refine {b | decides b (forall idx : BoundedIndex As, P idx)}
+             {b | decides b (@Iterate_Ensemble_BoundedIndex As P)}.
+  Proof.
+    intros; eapply refine_pick_pick.
+    intros; destruct x; simpl in *.
+    intros; eapply Iterate_Ensemble_equiv' with (Visited := []);
+    eauto using string_dec.
+    destruct n; simpl; intros; discriminate.
+    unfold not; intros; apply H.
+    apply Iterate_Ensemble_equiv'';
+      auto using string_dec.
+  Qed.
 
   Lemma QSInsertSpec_refine :
-    forall qsSchema qs idx tup default,
-      refine (Pick (QSInsertSpec {| qsHint := qs |} idx tup)) default
-      -> refine
-           (Pick (QSInsertSpec {| qsHint := qs |} idx tup))
-           (schConstr <- {b | b = true ->
-                              schemaConstraints (QSGetNRelSchema qsSchema idx) tup};
-            qsConstr <- {b | b = true ->
-                             (forall idx',
-                                BuildQueryStructureConstraints qsSchema idx idx' tup (GetRelation qs idx'))};
-            qsConstr' <- {b | b = true ->
-                              forall idx',
-                                idx' <> idx ->
-                                forall tup',
-                                  BuildQueryStructureConstraints qsSchema idx' idx tup'
-                                                                 (RelationInsert tup (GetRelation qs idx))};
+    forall qsSchema (qs : QueryStructure qsSchema) Ridx tup default,
+      refine
+           (Pick (QSInsertSpec {| qsHint := qs |} Ridx tup))
+           (schConstr <- {b | decides b (SatisfiesSchemaConstraints Ridx tup)};
+            qsConstr <- {b | decides b
+(forall Ridx', SatisfiesCrossRelationConstraints Ridx Ridx' tup (GetRelation qs Ridx'))};
+            qsConstr' <- {b | decides
+                                b
+                                (forall Ridx',
+                                   Ridx' <> Ridx ->
+                                   forall tup',
+                                     SatisfiesCrossRelationConstraints
+                                       Ridx' Ridx tup'
+                                       (RelationInsert tup (GetRelation qs Ridx)))};
             match schConstr, qsConstr, qsConstr' with
               | true, true, true =>
                 {qs' |
-                 (forall idx',
-                    idx <> idx' ->
-                    GetRelation qsHint idx' =
-                    GetRelation qs' idx')
+                 (forall Ridx',
+                    Ridx <> Ridx' ->
+                    GetRelation qsHint Ridx' =
+                    GetRelation qs' Ridx')
                  /\ forall t,
-                      GetRelation qs' idx t <->
-                      (RelationInsert tup (GetRelation qsHint idx) t)
+                      GetRelation qs' Ridx t <->
+                      (RelationInsert tup (GetRelation qsHint Ridx) t)
              }
 
               | _, _, _ => default
             end).
   Proof.
-    intros qsSchema qs idx tup default refines_default v Comp_v.
-    do 3 (apply_in_hyp computes_to_inv; destruct_ex; intuition);
-    destruct x; destruct x0; destruct x1; eauto.
-    repeat (apply_in_hyp computes_to_inv; destruct_ex; intuition).
-    econstructor; unfold QSInsertSpec; eauto.
+    intros qsSchema qs Ridx tup default v Comp_v.
+    do 3 (apply_in_hyp computes_to_inv; destruct_ex; split_and);
+      destruct x;
+      [ destruct x0;
+        [ destruct x1;
+          [ repeat (apply_in_hyp computes_to_inv; destruct_ex; split_and); simpl in *;
+            econstructor; unfold QSInsertSpec; eauto |
+             ]
+        |  ]
+      |  ];
+      cbv delta [decides] beta in *; simpl in *;
+      repeat (apply_in_hyp computes_to_inv; destruct_ex); eauto;
+      econstructor; unfold QSInsertSpec; intros;
+      elimtype False; intuition.
   Qed.
 
-  (*
-  Lemma refine_Any_DecideableSB_True
-  : refine (Any (DecideableSB True)) (ret (left I)).
+  (* So that things play nicely with setoid rewriting *)
+  Definition If_Then_Else {A}  (b : bool) (t e : A)
+    := if b then t else e.
+
+  Program Fixpoint Iterate_Decide_Comp' (A : Set)
+          (Remaining Visited : list A)
+          (P : Ensemble (BoundedIndex (Visited ++ Remaining)))
+          {struct Remaining }
+  : Comp bool :=
+    match Remaining with
+      | nil => ret true
+      | cons a Remaining' =>
+        Bind {b' |
+              decides b' (P {| bindex := a;
+                               indexb := {| ibound := List.length Visited;
+                                            boundi := _ |} |})}%comp
+             (fun b' =>
+                If_Then_Else b'
+                             (Iterate_Decide_Comp' Remaining' (Visited ++ [a]) _)
+                             (ret false))
+    end.
+  Next Obligation.
+    clear P; induction Visited; simpl; auto.
+  Defined.
+  Next Obligation.
+    exact (Ensemble_BoundedIndex_app_cons _ _ _ P).
+  Defined.
+
+  Lemma refine_Iterate_Decided_Ensemble' {A : Set}
+        (A_eq_dec : forall a a' : A, {a = a'} + {a <> a'})
+  : forall (Remaining Visited : list A)
+           (P : Ensemble (BoundedIndex (Visited ++ Remaining))),
+      refine {b | decides b (Iterate_Ensemble_BoundedIndex' Visited Remaining P)}
+             (Iterate_Decide_Comp' Remaining Visited P).
   Proof.
-    repeat constructor.
+    induction Remaining; simpl; intros.
+    - econstructor; inversion_by computes_to_inv; subst; simpl; auto.
+    - econstructor; apply computes_to_inv in H; destruct_ex;
+      split_and; inversion_by computes_to_inv; subst.
+      destruct x; simpl in *.
+      {  destruct v; simpl in *; intuition; intros; eauto.
+         - generalize (IHRemaining (Visited ++ [a]) _ _ H1).
+           intros; inversion_by computes_to_inv; simpl in *; eauto.
+         - generalize (IHRemaining (Visited ++ [a]) _ _ H1).
+           intros; inversion_by computes_to_inv; simpl in *; eauto.
+      }
+      { inversion_by computes_to_inv; subst; simpl; intuition. }
+  Qed.
+
+  Lemma decides_True :
+    refine {b | decides b True}%comp
+           (ret true).
+  Proof.
+    econstructor; inversion_by computes_to_inv; subst; simpl; auto.
+  Qed.
+
+  Lemma decides_2_True (A B : Type) :
+    refine {b' | decides b' (A -> B -> True)}%comp
+           (ret true).
+  Proof.
+    econstructor; inversion_by computes_to_inv; subst; simpl; auto.
+  Qed.
+
+  Lemma decides_neq (A : Type) (B : Prop) (a : A) :
+    refine {b' | decides b' (a <> a -> B)}%comp
+           (ret true).
+  Proof.
+    econstructor; inversion_by computes_to_inv; subst; simpl; auto.
+    congruence.
+  Qed.
+
+  Global Add Parametric Morphism A
+  : If_Then_Else
+      with signature
+      (@eq bool) ==> (@refine A) ==> (@refine A) ==> (@refine A)
+        as refine_if.
+  Proof.
+    compute.
+    intros; destruct_head bool; intros; eauto.
+  Qed.
+
+  Definition Iterate_Decide_Comp
+          (Bound : list string)
+          (P : Ensemble (BoundedIndex Bound))
+  : Comp bool :=
+    Iterate_Decide_Comp' Bound [] P.
+
+  Definition Iterate_Decide_Comp_BoundedIndex
+  : forall (Bound : list string)
+           (P : Ensemble (BoundedIndex Bound)),
+      refine {b | decides b (forall Ridx', P Ridx')}
+             (Iterate_Decide_Comp P).
+  Proof.
+    intros.
+    setoid_rewrite refine_Iterate_Ensemble; auto using string_dec.
+    setoid_rewrite refine_Iterate_Decided_Ensemble'; auto using string_dec.
+    reflexivity.
+  Qed.
+
+  (* Definition GetRelevantConstraints
+             qsSchema
+             Ridx
+  : list string :=
+    map (fun f => bindex (snd (projT1 f)))
+        (filter (fun f => if (BoundedIndex_eq_dec string_dec Ridx (fst (projT1 f)))
+                          then true
+                          else false)
+                (qschemaConstraints qsSchema)).
+
+  Definition lift_BoundedIndex
+             qsSchema Ridx
+             (Ridx' : BoundedIndex (GetRelevantConstraints qsSchema Ridx))
+  : BoundedString (map relName (qschemaSchemas qsSchema)).
+    destruct Ridx' as [Ridx' [n nth_n]];
+    econstructor 1 with (bindex := Ridx').
+    unfold GetRelevantConstraints in *.
+    revert n nth_n.
+    induction (qschemaConstraints qsSchema); simpl in *; intros.
+    - destruct n; discriminate.
+    - destruct n; simpl in *.
+      revert nth_n.
+      case_eq (BoundedIndex_eq_dec string_dec Ridx (fst (projT1 a)));
+        intros; subst.
+
+    econstructor; eauto.
+
+    intros
+
+
+  Lemma Iterate_Decide_Comp_refine :
+    forall qsSchema (qs : QueryStructure qsSchema) Ridx tup,
+      refine (@Iterate_Decide_Comp _
+                                   (fun Ridx' =>
+                                      SatisfiesCrossRelationConstraints
+                                        Ridx Ridx' tup
+                                        (GetRelation qs Ridx')))
+             (@Iterate_Decide_Comp (GetRelevantConstraints qsSchema Ridx)
+                                   (fun Ridx' =>
+                                      SatisfiesCrossRelationConstraints
+                                        Ridx Ridx' tup
+                                        (GetRelation qs Ridx'))).
+
+
+Definition SatisfiesCrossRelationConstraints
+           {qsSchema} Ridx Ridx' tup R :=
+  BuildQueryStructureConstraints qsSchema Ridx Ridx' tup R. *)
+
+
+  Lemma QSInsertSpec_refine' :
+    forall qsSchema (qs : QueryStructure qsSchema) Ridx tup default,
+      refine
+           (Pick (QSInsertSpec {| qsHint := qs |} Ridx tup))
+           (schConstr <- {b | decides b (SatisfiesSchemaConstraints Ridx tup)};
+            qsConstr <- (@Iterate_Decide_Comp _
+                                (fun Ridx' =>
+                                   SatisfiesCrossRelationConstraints
+                                     Ridx Ridx' tup
+                                     (GetRelation qsHint Ridx')));
+            qsConstr' <- (@Iterate_Decide_Comp _
+                                (fun Ridx' =>
+                                   Ridx' <> Ridx ->
+                                   forall tup',
+                                     SatisfiesCrossRelationConstraints
+                                       Ridx' Ridx tup'
+                                       (RelationInsert tup (GetRelation qs Ridx))));
+            match schConstr, qsConstr, qsConstr' with
+              | true, true, true =>
+                {qs' |
+                 (forall Ridx',
+                    Ridx <> Ridx' ->
+                    GetRelation qsHint Ridx' =
+                    GetRelation qs' Ridx')
+                 /\ forall t,
+                      GetRelation qs' Ridx t <->
+                      (RelationInsert tup (GetRelation qsHint Ridx) t)
+             }
+
+              | _, _, _ => default
+            end).
+  Proof.
+    intros.
+    rewrite QSInsertSpec_refine; f_equiv.
+    unfold pointwise_relation; intros.
+    rewrite Iterate_Decide_Comp_BoundedIndex; f_equiv.
+    unfold pointwise_relation; intros.
+    rewrite Iterate_Decide_Comp_BoundedIndex; reflexivity.
+  Qed.
+
+  (* Lemma Iterate_Ensemble_equiv {A : Set}
+        (A_eq_dec : forall a a' : A, {a = a'} + {a <> a'})
+  : forall (Remaining Visited : list A)
+           (P : Ensemble (BoundedIndex (Visited ++ Remaining))),
+      (forall a n (nth : nth_error Visited n = Some a),
+         P {| bindex := a;
+              indexb := {| ibound := n;
+                           boundi := nth_error_app _ _ _ nth |} |})
+      -> (Iterate_Ensemble_BoundedIndex Visited Remaining P ->
+         forall idx, P idx).
+    intros; destruct idx as [idx [n nth_n] ]; simpl in *.
+    revert Visited P H H0 idx n nth_n; induction Remaining; simpl; intros.
+    - eapply Ensemble_BoundedIndex_nth_eq with (a := idx); auto.
+    - split_and.
+      assert (nth_error ((Visited ++ [a]%SchemaConstraints) ++ Remaining) n = Some idx)
+        as nth_n'
+          by (rewrite <- app_assoc; simpl; assumption).
+      generalize (IHRemaining _ _ (Ensemble_nth_error_app A_eq_dec _ _ _ P H1 H) H2 _ _ nth_n').
+      unfold Ensemble_BoundedIndex_app_cons, eq_rect; destruct (app_cons a Visited Remaining).
+      intros; erewrite (eq_proofs_unicity_Opt_A A_eq_dec nth_n); eauto.
+      Grab Existential Variables.
+      rewrite app_nil_r in nth_n; assumption.
+  Qed.
+
+  Lemma Iterate_Ensemble_equiv' {A : Set}
+        (A_eq_dec : forall a a' : A, {a = a'} + {a <> a'})
+  : forall (Remaining Visited : list A)
+           (P : Ensemble (BoundedIndex (Visited ++ Remaining))),
+      (forall idx, P idx)
+      -> Iterate_Ensemble_BoundedIndex Visited Remaining P.
+    induction Remaining; simpl; auto.
+    intros; split; eauto.
+    eapply IHRemaining; intros; eauto.
+    intros; destruct idx as [idx [n nth_n] ]; simpl in *.
+    eapply Ensemble_BoundedIndex_app_equiv; eauto.
+    Grab Existential Variables.
+    rewrite <- app_assoc in nth_n; simpl in nth_n; eassumption.
+  Qed.
+
+  Lemma refine_Iterate_Ensemble {A : Set}
+        (A_eq_dec : forall a a' : A, {a = a'} + {a <> a'})
+  : forall (As : list A)
+           (P : Ensemble (BoundedIndex As)),
+      refine {b | decides b (forall idx, P idx)}
+             {b | decides b (Iterate_Ensemble_BoundedIndex [] As P)}.
+  Proof.
+    intros; eapply refine_pick_pick.
+    intros; destruct x; simpl in *.
+    intros; eapply Iterate_Ensemble_equiv with (Visited := []); eauto.
+    destruct n; simpl; intros; discriminate.
+    unfold not; intros; apply H.
+    apply Iterate_Ensemble_equiv'; auto.
+  Qed.
+
+
+
+  Lemma QSInsertSpec_refine :
+    forall qsSchema (qs : QueryStructure qsSchema) Ridx tup default,
+      refine
+           (Pick (QSInsertSpec {| qsHint := qs |} Ridx tup))
+           (schConstr <- {b | decides b (SatisfiesSchemaConstraints Ridx tup)};
+            qsConstr <- {b | decides b
+(forall Ridx', SatisfiesCrossRelationConstraints Ridx Ridx' tup (GetRelation qs Ridx'))};
+            qsConstr' <- {b | decides
+                                b
+                                (forall Ridx',
+                                   Ridx' <> Ridx ->
+                                   forall tup',
+                                     SatisfiesCrossRelationConstraints
+                                       Ridx' Ridx tup'
+                                       (RelationInsert tup (GetRelation qs Ridx)))};
+            match schConstr, qsConstr, qsConstr' with
+              | true, true, true =>
+                {qs' |
+                 (forall Ridx',
+                    Ridx <> Ridx' ->
+                    GetRelation qsHint Ridx' =
+                    GetRelation qs' Ridx')
+                 /\ forall t,
+                      GetRelation qs' Ridx t <->
+                      (RelationInsert tup (GetRelation qsHint Ridx) t)
+             }
+
+              | _, _, _ => default
+            end).
+  Proof.
+    intros qsSchema qs Ridx tup default v Comp_v.
+    do 3 (apply_in_hyp computes_to_inv; destruct_ex; split_and);
+      destruct x;
+      [ destruct x0;
+        [ destruct x1;
+          [ repeat (apply_in_hyp computes_to_inv; destruct_ex; split_and); simpl in *;
+            econstructor; unfold QSInsertSpec; eauto |
+             ]
+        |  ]
+      |  ];
+      cbv delta [decides] beta in *; simpl in *;
+      repeat (apply_in_hyp computes_to_inv; destruct_ex); eauto;
+      econstructor; unfold QSInsertSpec; intros;
+      elimtype False; intuition.
   Qed.
 
   (* Infrastructure for Inserting into QueryStructures built using
      BuildQueryStructure*)
 
   Program Fixpoint DecideableSB_Comp (A : Type)
-          (A_eq_dec : forall a a' : A, {a = a'} + {a <> a'})
           (Bound : list A)
           (P : Ensemble A)
-          (ValidBound : forall a, ~ List.In a Bound -> P a)
           {struct Bound}
-  : Comp (DecideableSB (forall a : A, P a)) :=
-    match Bound as Bound'
-          return (forall a, ~ List.In a Bound' -> P a)
-                 -> _ with
-      | nil => fun ValidBound' => ret (left (fun a => ValidBound' a (id)))
-      | cons a Bound' => fun ValidBound' =>
-                           (Bind (Any (DecideableSB (P a)))
-                                 (fun Pa =>
-                                    if Pa
+  : Comp bool :=
+    match Bound as Bound' with
+      | nil => ret true
+      | cons a Bound' => Bind {b' | decides b' (P a)}%comp
+                                 (fun b' =>
+                                    if b'
                                     then
-                                      (DecideableSB_Comp A_eq_dec Bound' P)
-                                        (fun a0 => if A_eq_dec a a0 then _ else _)
-                                    else ret (right (fun H' => _ (H' _)))))
-    end ValidBound.
-  Next Obligation.
-    apply ValidBound'; intuition.
-  Defined.
+                                      DecideableSB_Comp Bound' P
+                                    else ret false)
+    end.
+
+  (* Next Obligation.
+
+    destruct b'; destruct b; simpl in *; try discriminate.
+    destruct (A_eq_dec a a0).
+    -
+    Focus 2.
+    apply ValidBound'; tauto.
+  Defined. *)
+
+  Definition Iterate_Constraints_dec
+             qsSchema
+             (qs : QueryStructure qsSchema)
+             Ridx
+             (tup : Tuple (QSGetNRelSchemaHeading qsSchema Ridx))
+    := DecideableSB_Comp
+         (map (fun constr => snd (projT1 constr)) (qschemaConstraints qsSchema))
+         (fun Ridx' =>
+            BuildQueryStructureConstraints
+              qsSchema Ridx Ridx' tup (GetRelation qs Ridx')).
+
+  Lemma DecideableSB_Comp_refine :
+  forall qsSchema
+         (qs : QueryStructure qsSchema)
+         Ridx
+         (tup : Tuple (QSGetNRelSchemaHeading qsSchema Ridx)),
+      refine
+        {b | decides b (forall Ridx',
+                          SatisfiesCrossRelationConstraints Ridx Ridx' tup (GetRelation qs Ridx')) }
+      (Iterate_Constraints_dec qs Ridx tup).
+  Proof.
+    unfold Iterate_Constraints_dec, SatisfiesCrossRelationConstraints,
+    QSGetNRelSchema; simpl.
+    unfold BuildQueryStructureConstraints.
+    intro; induction (qschemaConstraints qsSchema); simpl; intros.
+    - repeat econstructor; inversion_by computes_to_inv; subst; simpl; auto.
+    - intros v Comp_v; apply computes_to_inv in Comp_v; destruct_ex; split_and.
+      destruct x.
+      generalize (IHl _ _ _ _ H1).
+      econstructor.
+      unfold BuildQueryStructureConstraints_cons; simpl.
+      destruct (Peano_dec.eq_nat_dec (ibound Ridx) (ibound (fst (projT1 a)))).
+      simpl.
+
+    intros.
+    repeat econstructor.
+
+  Qed.
+
+  Definition Iterate_Constraints_dec'
+             qsSchema
+             (qs : QueryStructure qsSchema)
+             Ridx
+             (tup : Tuple (QSGetNRelSchemaHeading qsSchema Ridx))
+    := DecideableSB_Comp
+         string_dec
+         (map relName (qschemaSchemas qsSchema))
+         (fun Ridx' =>
+            Ridx' <> Ridx ->
+            forall tup' : Tuple (QSGetNRelSchemaHeading qsSchema Ridx'),
+            BuildQueryStructureConstraints
+              qsSchema Ridx' Ridx tup' (tup :: (GetRelation qs Ridx)))
+         (ValidBound_DecideableSB_Comp' qsSchema _ tup ).
+
+  Lemma DecideableSB_Comp'_refine :
+  forall qsSchema
+         (qs : QueryStructure qsSchema)
+         Ridx
+         (tup : Tuple (QSGetNRelSchemaHeading qsSchema Ridx)),
+      refine
+      (Any (QSSchemaConstraints_dec' qs Ridx tup))
+      (Iterate_Constraints_dec' qs Ridx tup).
+  Proof.
+    intros.
+    repeat econstructor.
+  Qed.
 
   Definition ValidBound_DecideableSB_Comp
              qsSchema
-             (qs : forall idx : string,
+             (qs : forall Ridx : string,
                      list
                        (Tuple
-                          (QSGetNRelSchemaHeading qsSchema idx)))
-             idx
-             (tup : Tuple (QSGetNRelSchemaHeading qsSchema idx))
+                          (QSGetNRelSchemaHeading qsSchema Ridx)))
+             Ridx
+             (tup : Tuple (QSGetNRelSchemaHeading qsSchema Ridx))
   : forall a : string,
       ~ List.In a (map relName (qschemaSchemas qsSchema)) ->
-      (fun idx' : string =>
+      (fun Ridx' : string =>
          BuildQueryStructureConstraints qsSchema
-           idx idx' tup (qs idx')) a.
+           Ridx Ridx' tup (qs Ridx')) a.
   Proof.
     destruct qsSchema as [namedSchemas constraints]; simpl in *.
     simpl in *; induction constraints;
@@ -230,7 +831,7 @@ Section InsertRefinements.
     BuildQueryStructureConstraints_cons,
     BuildQueryStructureConstraints_cons_obligation_1 in *;
       simpl in *.
-    destruct (string_dec s idx); try (apply IHconstraints; eauto; fail).
+    destruct (string_dec s Ridx); try (apply IHconstraints; eauto; fail).
     destruct (string_dec s0 a0); try (apply IHconstraints; eauto; fail).
     destruct e; destruct e0.
     unfold eq_sym, eq_rect; simpl.
@@ -240,19 +841,19 @@ Section InsertRefinements.
 
   Definition ValidBound_DecideableSB_Comp'
              qsSchema
-             (qs : forall idx : string,
+             (qs : forall Ridx : string,
                      list
                        (Tuple
-                          (QSGetNRelSchemaHeading qsSchema idx)))
-             idx
-             (tup : Tuple (QSGetNRelSchemaHeading qsSchema idx))
+                          (QSGetNRelSchemaHeading qsSchema Ridx)))
+             Ridx
+             (tup : Tuple (QSGetNRelSchemaHeading qsSchema Ridx))
   : forall a : string,
       ~ List.In a (map relName (qschemaSchemas qsSchema)) ->
-      a <> idx ->
+      a <> Ridx ->
       forall
         tup' : Tuple (QSGetNRelSchemaHeading qsSchema a),
         BuildQueryStructureConstraints qsSchema
-                                       a idx tup' (tup :: qs idx).
+                                       a Ridx tup' (tup :: qs Ridx).
   Proof.
     destruct qsSchema as [namedSchemas constraints]; simpl in *.
     simpl in *; induction constraints;
@@ -263,7 +864,7 @@ Section InsertRefinements.
     BuildQueryStructureConstraints_cons_obligation_1 in *;
       simpl in *.
     destruct (string_dec s a0); try (apply IHconstraints; eauto; fail).
-    destruct (string_dec s0 idx); try (apply IHconstraints; eauto; fail).
+    destruct (string_dec s0 Ridx); try (apply IHconstraints; eauto; fail).
     destruct e; destruct e0.
     unfold eq_sym, eq_rect; simpl.
     destruct (in_dec string_dec s (map relName namedSchemas)); auto.
@@ -273,27 +874,27 @@ Section InsertRefinements.
   Definition Iterate_Constraints_dec
              qsSchema
              (qs : QueryStructure qsSchema)
-             idx
-             (tup : Tuple (QSGetNRelSchemaHeading qsSchema idx))
+             Ridx
+             (tup : Tuple (QSGetNRelSchemaHeading qsSchema Ridx))
     := DecideableSB_Comp
          string_dec
          (map relName (qschemaSchemas qsSchema))
-         (fun idx' =>
+         (fun Ridx' =>
             BuildQueryStructureConstraints
-              qsSchema idx idx' tup (GetRelation qs idx'))
+              qsSchema Ridx Ridx' tup (GetRelation qs Ridx'))
          (ValidBound_DecideableSB_Comp qsSchema _
-                                       idx tup ).
+                                       Ridx tup ).
 
   Set Printing All.
 
   Lemma DecideableSB_Comp_refine :
   forall qsSchema
          (qs : QueryStructure qsSchema)
-         idx
-         (tup : Tuple (QSGetNRelSchemaHeading qsSchema idx)),
+         Ridx
+         (tup : Tuple (QSGetNRelSchemaHeading qsSchema Ridx)),
       refine
-      (Any (QSSchemaConstraints_dec qs idx tup))
-      (Iterate_Constraints_dec qs idx tup).
+      (Any (QSSchemaConstraints_dec qs Ridx tup))
+      (Iterate_Constraints_dec qs Ridx tup).
   Proof.
     intros.
     repeat econstructor.
@@ -302,26 +903,26 @@ Section InsertRefinements.
   Definition Iterate_Constraints_dec'
              qsSchema
              (qs : QueryStructure qsSchema)
-             idx
-             (tup : Tuple (QSGetNRelSchemaHeading qsSchema idx))
+             Ridx
+             (tup : Tuple (QSGetNRelSchemaHeading qsSchema Ridx))
     := DecideableSB_Comp
          string_dec
          (map relName (qschemaSchemas qsSchema))
-         (fun idx' =>
-            idx' <> idx ->
-            forall tup' : Tuple (QSGetNRelSchemaHeading qsSchema idx'),
+         (fun Ridx' =>
+            Ridx' <> Ridx ->
+            forall tup' : Tuple (QSGetNRelSchemaHeading qsSchema Ridx'),
             BuildQueryStructureConstraints
-              qsSchema idx' idx tup' (tup :: (GetRelation qs idx)))
+              qsSchema Ridx' Ridx tup' (tup :: (GetRelation qs Ridx)))
          (ValidBound_DecideableSB_Comp' qsSchema _ tup ).
 
   Lemma DecideableSB_Comp'_refine :
   forall qsSchema
          (qs : QueryStructure qsSchema)
-         idx
-         (tup : Tuple (QSGetNRelSchemaHeading qsSchema idx)),
+         Ridx
+         (tup : Tuple (QSGetNRelSchemaHeading qsSchema Ridx)),
       refine
-      (Any (QSSchemaConstraints_dec' qs idx tup))
-      (Iterate_Constraints_dec' qs idx tup).
+      (Any (QSSchemaConstraints_dec' qs Ridx tup))
+      (Iterate_Constraints_dec' qs Ridx tup).
   Proof.
     intros.
     repeat econstructor.
@@ -330,12 +931,12 @@ Section InsertRefinements.
   Lemma QSInsertSpec_BuildQuerySpec_refine :
     forall qsSchema
            (qs : QueryStructure qsSchema)
-           idx tup default,
+           Ridx tup default,
       refine
-        (Pick (QSInsertSpec {| qsHint := qs |} idx tup))
-        (schConstr <- Any (SchemaConstraints_dec _ idx tup);
-         qsConstr <- (Iterate_Constraints_dec qs idx tup);
-         qsConstr' <- (Iterate_Constraints_dec' qs idx tup);
+        (Pick (QSInsertSpec {| qsHint := qs |} Ridx tup))
+        (schConstr <- Any (SchemaConstraints_dec _ Ridx tup);
+         qsConstr <- (Iterate_Constraints_dec qs Ridx tup);
+         qsConstr' <- (Iterate_Constraints_dec' qs Ridx tup);
          match schConstr, qsConstr, qsConstr' with
            | left schConstr, left qsConstr, left qsConstr' =>
              ret (Insert_Valid qs tup schConstr qsConstr qsConstr')
